theories/reflect/progdef.v
@@ -9,94 +9,61 @@ From stdpp Require Import base strings gmap stringmap fin_maps.
 From iris.proofmode Require Import tactics.
 From shack Require Import lang progdef.
 
-Section Extends.
+Section SolveAcc.
   (* assume a given set of class definitions *)
   Context `{PDC: ProgDefContext}.
 
-  Definition extendsb A B : bool :=
-    if pdefs !! A is Some adef then
-    if adef.(superclass) is Some (t, _) then String.eqb B t else false
+  Fixpoint check_acc_def n c : bool :=
+    if n is S p then
+      if pdefs !! c is Some cdef then
+        if cdef.(superclass) is Some (parent, _) then
+          if pdefs !! parent is Some pdef then
+            check_acc_def p parent
+          else false
+        else true
+      else false
     else false
-  .
+.
 
-  Lemma extendsb_correct A B : extendsb A B ↔ extends A B.
+  Lemma check_acc_def_correct n:
+    ∀ c, check_acc_def n c → Acc (λ x y, extends y x) c.
   Proof.
-    rewrite /extendsb; split.
-    - destruct (pdefs !! A) as [adef | ] eqn:hadef; last done.
-      destruct (adef.(superclass)) as [(t, ?) | ] eqn:hsuper; last done.
-      move => heq.
-      destruct (B =? t) eqn:h; last done.
-      apply String.eqb_eq in h; subst.
-      by econstructor.
-    - move => h; destruct h as [A B adef σ hadef hsuper].
-      rewrite hadef hsuper.
-      destruct (B =? B) eqn:h; first done.
-      by rewrite eqb_neq in h.
-  Qed.
-End Extends.
-
-Lemma pacc_helper (P: tag → Prop) (xdefs: stringmap classDef):
-  Forall P (map fst (map_to_list xdefs)) →
-  Forall (uncurry (λ c _, P c)) (map_to_list xdefs).
-Proof.
-  rewrite Forall_lookup => h.
-  rewrite Forall_lookup => k [c ?] hk /=.
-  apply h with k.
-  by rewrite list_lookup_fmap hk.
-Qed.
-
-(* Helper tactics to deal with the `Acc` goal in progdef.v *)
-Lemma string_eqb_correct (s t: string) : (s =? t)%string ↔ s = t.
-Proof.
-  destruct String.eqb eqn:h.
-  - by apply String.eqb_eq in h as ->.
-  - apply String.eqb_neq in h.
-    by split.
-Qed.
-
-(* Do one step of Accessibility *)
-Ltac simpl_acc0 :=
-  constructor => ? /extendsb_correct;
-  rewrite /extendsb /=;
-  simpl_map => /=.
-
-(* If the previous tactic didn't solve the goal,
- * rewrite.
- *)
-Ltac simpl_acc1 := move/string_eqb_correct => ->.
-
-(* Gluing both tactics into an automated one *)
-Ltac simpl_acc_match :=
-  match goal with
-  | |- False → _ => done
-  | |- _ => (simpl_acc1; simpl_acc0)
-  end.
-
-Ltac simpl_acc := simpl_acc0; repeat simpl_acc_match.
-
-Ltac step_pacc :=
-  match goal with
-  | |- None = Some ?t → _ => done
-  | H : nat |- _ => destruct H; first (case => <-; simpl_acc)
-  end.
-
-Definition pacc_uncurry_def `{PDC: ProgDefContext} :=
-  Forall (uncurry (λ c _, Acc (λ x y : tag, extends y x) c))
-         (map_to_list pdefs).
-
-Lemma pacc `{PDC: ProgDefContext}:
-  pacc_uncurry_def → ∀ c, Acc (λ x y : tag, extends y x) c.
-Proof.
-  move => hacc.
-  assert (pacc_ : map_Forall (λ c _, Acc (λ x y, extends y x) c) pdefs).
-  { rewrite map_Forall_to_list /=.
-    by apply hacc.
-  }
-  move => c.
-  destruct (pdefs !! c) as [cdef | ] eqn:hcdef.
-  - move : pacc_ => /map_Forall_lookup h.
-    by eapply h.
-  - constructor => t hext; exfalso.
-    inv hext.
+    elim: n => [ // | p ] /= hi c.
+    destruct (pdefs !! c) as [cdef | ] eqn:hcdef; last done.
+    destruct (cdef.(superclass)) as [ [parent ?] | ] eqn:hsuper; last first.
+    { move => _; constructor => ? h.
+      destruct h as [A B adef σ hadef' hsuper'].
+      by simplify_eq.
+    }
+    destruct (pdefs !! parent); last done.
+    move/hi => hacc.
+    constructor => ? h.
+    destruct h as [A B adef σ hadef' hsuper'].
     by simplify_eq.
-Qed.
+  Qed.
+
+  Definition check_acc_defs n : bool :=
+    forallb (λ kv, check_acc_def n kv.1) (map_to_list pdefs).
+
+  Lemma check_acc_defs_correct n:
+    check_acc_defs n →
+    ∀ c, Acc (λ x y, extends y x) c.
+  Proof.
+    assert (hForall:
+      check_acc_defs n → map_Forall (λ c _, Acc (λ x y, extends y x) c) pdefs).
+    { rewrite map_Forall_to_list /check_acc_defs forallb_True Forall_lookup.
+      rewrite Forall_lookup => h k [c cdef] hcdef /=.
+      apply check_acc_def_correct with n.
+      by apply h in hcdef.
+    }
+    move => h.
+    move: {hForall h} (hForall h).
+    rewrite map_Forall_lookup => h c.
+    destruct (pdefs !! c) as [cdef | ] eqn:hcdef; last first.
+    { constructor => ? hext.
+      destruct hext as [].
+      by simplify_eq.
+    }
+    by apply h in hcdef.
+  Qed.
+End SolveAcc.
